pancake/pan_to_wordScript.sml
@@ -1,0 +1,20 @@
+(*
+  Correctness proof for --
+*)
+
+open preamble
+     pan_to_crepTheory crep_to_loopTheory
+     loop_to_wordTheory
+
+val _ = new_theory "pan_to_word";
+
+
+Definition compile_prog:
+  compile_prog prog =
+  let prog = pan_to_crep$compile_prog prog;
+      prog = crep_to_loop$compile_prog prog in
+    loop_to_word$compile prog
+End
+
+
+val _ = export_theory();
