pancake/proofs/pan_to_wordProofScript.sml
@@ -1,0 +1,123 @@
+(*
+  Correctness proof for --
+*)
+
+open preamble pan_to_wordTheory
+     pan_to_crepProofTheory crep_to_loopProofTheory
+     loop_to_wordProofTheory
+
+val _ = new_theory "pan_to_wordProof";
+
+
+Definition crep_state_def:
+  crep_state (s:('a,'ffi) panSem$state) (pan_code:(mlstring # (mlstring # shape) list # α prog) list) =
+  <| locals   := FEMPTY;
+     globals  := FEMPTY;
+     code     := alist_to_fmap (pan_to_crep$compile_prog pan_code);
+     eids     := FRANGE ((get_eids pan_code):mlstring |-> 'a word);
+     memory   := s.memory;
+     memaddrs := s.memaddrs;
+     clock    := s.clock;
+     be       := s.be;
+     ffi      := s.ffi|>
+End
+
+
+Definition mk_mem_def:
+  mk_mem ctxt smem =
+        λad. wlab_wloc ctxt (smem ad)
+End
+
+Definition loop_state_def:
+  loop_state (s:('a,'ffi) crepSem$state) crep_code =
+  let ctxt = mk_ctxt FEMPTY (make_funcs crep_code) 0 (get_eids crep_code) in
+  <| locals   := LN;
+     globals  := FEMPTY;
+     memory   := mk_mem ctxt s.memory;
+     mdomain := s.memaddrs;
+     code     := fromAList (crep_to_loop$compile_prog crep_code);
+     clock    := ARB;
+     be       := s.be;
+     ffi      := s.ffi|>
+End
+
+Theorem get_eids_equivs:
+   !pan_code. equivs (FRANGE ((get_eids pan_code):mlstring |-> 'a word))
+          ((get_eids (compile_prog pan_code)): 'a word set)
+Proof
+  cheat
+
+QED
+
+Theorem all_distinct_first_compile_prog:
+  ALL_DISTINCT (MAP FST pan_code) ==>
+  ALL_DISTINCT (MAP FST (pan_to_crep$compile_prog pan_code))
+Proof
+  cheat
+QED
+
+Theorem alookup_compile_prog_code:
+  ALOOKUP pan_code start = SOME ([],prog) ==>
+  ALOOKUP (pan_to_crep$compile_prog pan_code) start =
+  SOME ([],
+        comp_func (make_funcs pan_code) (get_eids pan_code) [] prog)
+Proof
+  cheat
+QED
+
+
+Theorem state_rel_imp_semantics:
+  s.memaddrs = t.mdomain ∧
+  s.be = t.be ∧
+  s.ffi = t.ffi ∧
+  ALL_DISTINCT (MAP FST pan_code) ∧
+  s.code = alist_to_fmap pan_code ∧
+  t.code = fromAList (pan_to_word$compile_prog pan_code) ∧
+  s.locals = FEMPTY ∧ size_of_eids pan_code < dimword (:α) ∧
+  FDOM s.eshapes = FDOM ((get_eids pan_code):mlstring |-> 'a word) ∧
+  (∀ad f.
+   s.memory ad = Label f ⇒
+   ∃n m. FLOOKUP (make_funcs (compile_prog pan_code)) f = SOME (n,m)) /\
+  ALOOKUP pan_code start = SOME ([],prog) ∧
+  semantics s start <> Fail ==>
+  semantics (t:('a,'b, 'ffi) wordSem$state) lc =
+  semantics (s:('a,'ffi) panSem$state) start
+Proof
+  rw [] >>
+  ‘state_rel s (crep_state s pan_code)’ by (
+    fs [pan_to_crepProofTheory.state_rel_def, crep_state_def]) >>
+  drule pan_to_crepProofTheory.state_rel_imp_semantics >>
+  disch_then (qspecl_then [‘start’, ‘prog’ , ‘pan_code’] mp_tac) >>
+  fs [] >>
+  impl_tac
+  >- fs [crep_state_def] >>
+  strip_tac >>
+  pop_assum (assume_tac o GSYM) >>
+  fs [] >>
+  ‘(crep_state s pan_code).memaddrs =
+   (loop_state (crep_state s pan_code) (pan_to_crep$compile_prog pan_code)).mdomain’ by
+    fs [crep_state_def, loop_state_def] >>
+  drule crep_to_loopProofTheory.state_rel_imp_semantics >>
+  disch_then (qspecl_then [‘start’, ‘comp_func (make_funcs pan_code) (get_eids pan_code) [] prog’,
+                           ‘lc’, ‘compile_prog pan_code’] mp_tac) >>
+  impl_tac
+  >- (
+   fs [crep_state_def, loop_state_def] >>
+   conj_tac
+   >- (
+    fs [crep_to_loopTheory.mk_ctxt_def, mk_mem_def, mem_rel_def] >>
+    rw [] >> res_tac >> rfs []) >>
+   conj_tac
+   >- fs [get_eids_equivs] >>
+   conj_tac >- fs [crep_to_loopProofTheory.globals_rel_def] >>
+   conj_tac >- metis_tac [all_distinct_first_compile_prog] >>
+   conj_tac >- metis_tac [alookup_compile_prog_code] >>
+   cheat) >>
+  strip_tac >>
+  pop_assum (assume_tac o GSYM) >>
+  fs [] >>
+  pop_assum kall_tac >>
+  match_mp_tac fstate_rel_imp_semantics >>
+  cheat
+QED
+val _ = export_theory();
